\section{Rules for the Quantifiers}

\begin{Exercise}[number=18]
  Show, using $\forall$-introduction and Deduction Rule: if from $\Gamma$, $P(c)$ it follows that $Q(c)$ (where $c$ satisfies $P$, but is otherwise ``arbitrary''), then from $\Gamma$ it follows that $\forall{x} \colon P(x) \implies Q(x)$.
\end{Exercise}

\begin{Answer} [number=18]
  \begin{structured_derivation}
    \task{Prove $\Gamma \implies \bigl( \forall{x} \colon P(x) \implies Q(x) \bigr)$ provided that:}
    \assumption{$\bigl( P(c) \land \Gamma \bigr) \implies Q(c)$}
    \isProvedBy{deduction rule; suppose $\Gamma$ (because it's the antecedent)}
    \begin{nested_derivation}
      \task{Prove $\forall{x} \colon P(x) \implies Q(x)$ when:}
      \assumption{$\Gamma$}
      \isProvedBy{deduction rule}
      \begin{nested_derivation}
        \task{Prove $Q(x)$ when:}
        \assumption{$\exists{x} \suchthat P(x)$}
        \observation
          {A conjunction follows from its two conjuncts taken together.}
          { $\Gamma \land P(x)$ }
        \observation
          {\term{modus ponens}}
          { $Q(x)$ }
      \end{nested_derivation}
      \andbutso{$\forall{x} \colon P(x) \implies Q(x)$}
    \end{nested_derivation}
  \end{structured_derivation}
\end{Answer}